size <-> last_index

heap/tree_pop.v
@@ -4,7 +4,7 @@ Require Import Notations Logic Datatypes.
 From Coq Require Import String List ZArith. 
 From compcert Require Import Coqlib Integers Floats AST Ctypes Cop Clight Clightdefs.
 Require Import Coq.Logic.Classical_Pred_Type.
-Require Import Coq.Logic.Classical_Prop.
+Require Import Classical_Prop.
 
 Require Import Coq.micromega.Psatz.
 Local Open Scope string.
@@ -14,9 +14,487 @@ Local Open Scope list_scope.
 Require Import cprogs.heap.list_relation.
 Require Import cprogs.heap.definitions.
 Require Import cprogs.heap.tree_list.
-Require Import cprogs.heap.math_prop.
 Require Import cprogs.heap.tree_down.
+Require Import cprogs.heap.math_prop.
 
-Require Import SetsClass.SetsClass.
-Local Open Scope sets.
-Import SetsNotation.
+Fixpoint tree_to_partial_tree_pop_fix (tl: partial_tree) (t: tree) (d: Z): partial_tree :=
+  match t with
+    | Leaf => tl
+    | Node v ls rs => 
+      match (full_tree_b (d - 2) rs) with
+      | false => tree_to_partial_tree_pop_fix ((true, v, ls) :: tl) rs (d-1)
+      | true => tree_to_partial_tree_pop_fix ((false, v, rs) :: tl) ls (d-1)
+      end (*true go right and right is cut*)
+  end.
+
+Definition tree_to_partial_tree_pop(t: tree) (d: Z): partial_tree := 
+  tree_to_partial_tree_pop_fix nil t d.
+
+Definition get_last_val(l: partial_tree): Z :=
+  match l with
+    | nil => 0
+    | (flg, v, tr)::lt => v
+  end.
+
+Definition tree_cut_last(ls rs: tree) (d: Z): tree :=
+  if (full_tree_b (d - 2) rs) then
+    (Node (get_last_val (tree_to_partial_tree_pop ls (d-1)))
+        (tree_compose (skipn 1%nat (tree_to_partial_tree_pop ls (d-1))) Leaf) rs)
+  else (Node (get_last_val ( tree_to_partial_tree_pop rs (d-1)))
+        ls (tree_compose (skipn 1%nat (tree_to_partial_tree_pop rs (d-1))) Leaf)).
+
+Definition tree_pop: tree -> tree -> Prop :=
+  fun t t' => (tree_size t <= 1  /\ t' = Leaf) \/ 
+    (exists v ls rs ts d, t = (Node v ls rs) /\ complete_tree_pop d t /\ heap_tree_down (nil,(tree_cut_last ls rs d)) ts /\ t' = (tree_compose (fst ts) (snd ts))).
+
+Lemma complete_tree_pop_not_fullb: forall d t,
+  complete_tree_pop d t -> full_tree_b (d - 1) t = false.
+Proof.
+  intros.
+  induction H; subst; simpl.
+  + reflexivity.
+  + apply andb_false_intro1; auto.
+  + apply andb_false_intro2; auto.
+Qed.
+
+Fixpoint tree_last_pow2 (d: Z) (tr: tree): Z :=
+  match tr with
+    | Leaf => 1
+    | Node v ls rs =>
+      if (full_tree_b (d - 2) rs) then
+        2 * (tree_last_pow2 (d - 1) ls)
+      else
+        2 * (tree_last_pow2 (d - 1) rs) 
+  end.
+
+Lemma last_index_lowbit: forall d n tr,
+  complete_tree_pop d tr -> 
+  last_index d n tr = n * (tree_last_pow2 d tr) / 2 + last_index d 0 tr.
+Proof.
+  intros.
+  revert d n H.
+  induction tr; simpl; intros.
+  + rewrite Zdiv_0_l.
+    replace (n * 1) with n by lia. 
+    lia.
+  + inversion H; subst; simpl.
+    - rewrite full_tree_equiv1 in H4.
+      rewrite H4.
+      erewrite IHtr1; eauto.
+      rewrite Z.mul_assoc.
+      lia.
+    - pose proof complete_tree_pop_not_fullb _ _ H4.
+      replace (d - 1 - 1) with (d - 2) in H0 by lia.
+      rewrite H0.
+      erewrite IHtr2; eauto.
+      rewrite Z.mul_assoc.
+      specialize (IHtr2 _ 1 H4).
+      rewrite IHtr2.
+      destruct (classic (Zodd (tree_last_pow2 (d - 1) tr2))).
+      * pose proof Zodd_2p_plus_1 n.
+        replace (n * 2) with (2 * n) by lia. 
+        pose proof Zodd_mult_Zodd _ _ H3 H1.
+        pose proof Zodd_div2 _ H5.
+        replace (2 * n * tree_last_pow2 (d - 1) tr2) with (n * tree_last_pow2 (d - 1) tr2 * 2) by lia.
+        rewrite Z.div_mul by lia.
+        assert (Zodd 1). {
+          rewrite <- Zodd_bool_iff; auto.
+        }
+        pose proof Zodd_mult_Zodd _ _ H7 H1.
+        pose proof Zodd_div2 _ H8.
+        lia.
+      * pose proof Zeven_odd_dec (tree_last_pow2 (d - 1) tr2).
+        assert (Zeven (tree_last_pow2 (d - 1) tr2)). {
+          destruct H3; auto.
+          exfalso.
+          auto.
+        }
+        pose proof Zeven_mult_Zeven_r (n * 2 + 1) _ H5.
+        pose proof Zeven_div2 _ H6.
+        replace (n * 2 * tree_last_pow2 (d - 1) tr2) with (n * tree_last_pow2 (d - 1) tr2 * 2) by lia.
+        rewrite Z.div_mul by lia.
+        replace (1 * tree_last_pow2 (d - 1) tr2) with (tree_last_pow2 (d - 1) tr2) by lia.
+        pose proof Zeven_div2 _ H5.
+        lia.
+Qed.
+
+Lemma tree_last_pow2_even: forall tr d,
+  tr <> Leaf ->
+  tree_last_pow2 d tr = 2 * (tree_last_pow2 d tr / 2).
+Proof.
+  intros tr.
+  induction tr; simpl; intros; [contradiction |].
+  destruct (full_tree_b (d - 2) tr2) eqn:?.
+  + replace (2 * tree_last_pow2 (d - 1) tr1) with (tree_last_pow2 (d - 1) tr1 * 2) by lia.
+    rewrite Z.div_mul by lia.
+    lia.
+  + replace (2 * tree_last_pow2 (d - 1) tr2) with (tree_last_pow2 (d - 1) tr2 * 2) by lia.
+    rewrite Z.div_mul by lia.
+    lia.
+Qed.
+
+Lemma full_tree_b_dep_restrict_less: forall tr d,
+  full_tree_b d tr = true ->
+  full_tree_b (d - 1) tr = false.
+Proof.
+  intros tr.
+  induction tr; simpl; intros.
+  + rewrite Z.eqb_neq; rewrite Z.eqb_eq in H; lia.
+  + apply andb_prop in H; destruct H.
+    specialize (IHtr1 _ H).
+    apply andb_false_intro1; assumption. 
+Qed.
+
+Lemma full_tree_last_pow2: forall tr d,
+  full_tree d tr -> tree_last_pow2 d tr = tree_size tr + 1.
+Proof.
+  intros.
+  induction H; subst; simpl.
+  + lia.
+  + remember H0 as H0'; clear HeqH0'.
+    rewrite full_tree_equiv1 in H0.
+    apply full_tree_b_dep_restrict_less in H0.
+    replace (dep - 1 - 1) with (dep - 2) in H0 by lia.
+    rewrite H0.
+    rewrite (full_tree_same_size _ _ _ H H0').
+    lia.
+Qed.
+
+Lemma complete_tree_pop_nonneg: forall tr d,
+  complete_tree_pop d tr -> 0 <= d.
+Proof.
+  intros.
+  induction H; subst; simpl; lia.
+Qed.
+
+Lemma complete_tree_pop_last_pow2: forall tr d,
+  complete_tree_pop d tr ->
+  tree_last_pow2 d tr = 2 ^ d.
+Proof.
+  intros.
+  induction H; subst; simpl.
+  + reflexivity.
+  + rewrite full_tree_equiv1 in H0.
+    rewrite H0.
+    rewrite IHcomplete_tree_pop; eauto.
+    pose proof complete_tree_pop_nonneg _ _ H.
+    replace dep with (dep - 1 + 1) at 2 by lia.
+    rewrite Zpower_exp by lia.
+    lia.
+  + pose proof complete_tree_pop_not_fullb _ _ H0.
+    replace (dep - 1 - 1) with (dep - 2) in H1 by lia.
+    rewrite H1.
+    rewrite IHcomplete_tree_pop; eauto.
+    replace dep with (dep - 1 + 1) at 2 by lia.
+    pose proof complete_tree_pop_nonneg _ _ H0.
+    rewrite Zpower_exp by lia.
+    lia. 
+Qed.
+
+Lemma tree_last_index_size: forall tr d,
+  complete_tree_pop d tr -> 
+  last_index d 1 tr = tree_size tr.
+Proof.
+  intros tr.
+  induction tr; simpl; intros.
+  + rewrite Z.div_1_l by lia; lia.
+  + inversion H; subst.
+    - rewrite full_tree_equiv1 in H4.
+      rewrite H4.
+      erewrite last_index_lowbit; eauto.
+      specialize (IHtr1 _ H2).
+      erewrite last_index_lowbit in IHtr1; eauto.
+      destruct (classic (tr1 = Leaf)).
+      * subst; simpl.
+        inversion H2.
+        rewrite <- full_tree_equiv1 in H4.
+        pose proof full_tree_nonneg _ _ H4.
+        lia.
+      * replace (2 * tree_last_pow2 (d - 1) tr1) with (tree_last_pow2 (d - 1) tr1 * 2) by lia.
+        rewrite Z.div_mul by lia.
+        pose proof tree_last_pow2_even _ (d - 1) H0.
+        pose proof complete_tree_pop_last_pow2 _ _ H2.
+        rewrite <- full_tree_equiv1 in H4.
+        pose proof full_tree_size _ _ H4.
+        pose proof full_tree_nonneg _ _ H4.
+        replace (d - 1) with (d - 2 + 1) in H3 by lia.
+        rewrite Zpower_exp in H3 by lia.
+        replace (d - 2 + 1) with (d - 1) in H3 by lia.
+        rewrite H3, !H5; rewrite <- IHtr1.
+        replace (2 ^ 1) with 2 by lia.
+        replace (2 ^ 1) with 2 in H3 by lia. 
+        rewrite H3. 
+        rewrite Z.mul_assoc, Z.div_mul by lia.
+        lia.
+    - pose proof complete_tree_pop_not_fullb _ _ H4.
+      replace (d - 1 - 1) with (d - 2) in H0 by lia.
+      rewrite H0.
+      erewrite last_index_lowbit; eauto.
+      specialize (IHtr2 _ H4).
+      erewrite last_index_lowbit in IHtr2; eauto.
+      destruct (classic (tr2 = Leaf)).
+      * subst; simpl.
+        inversion H4.
+        inversion H2; subst; simpl; auto.
+        pose proof full_tree_nonneg _ _ H5; lia.
+      * pose proof tree_last_pow2_even _ (d - 1) H1.
+        rewrite <- IHtr2.
+        pose proof full_tree_size _ _ H2; rewrite H5.
+        pose proof complete_tree_pop_last_pow2 _ _ H4.
+        rewrite H6.
+        rewrite H6 in H3.
+        replace (2 * (2 ^ (d - 1) / 2)) with ((2 ^ (d - 1) / 2) * 2) in H3 by lia.
+        rewrite H3, !Z.mul_assoc, !Z.div_mul by lia.
+        lia.
+Qed.
+
+Lemma list_on_tree_last_val: forall l pt tr d n,
+  Zlength l > 2 -> list_on_tree_state (l, n) (pt, tr) ->
+  complete_tree_pop d tr ->
+  get_last_val (tree_to_partial_tree_pop_fix pt tr d) = Znth (last_index d n tr) l.
+Proof.
+  intros.
+  revert l pt n d H H0 H1.
+  induction tr; simpl; intros.
+  + unfold list_on_tree_state in H0; simpl in H0.
+    unfold list_on_tree_state_fix in H0; simpl in H0.
+    destruct H0 as [? [? [? [? ?]]]].
+    inversion H2; subst; simpl.
+    - simpl in H3; lia.
+    - reflexivity.
+  + unfold list_on_tree_state in H0; simpl in H0.
+    unfold list_on_tree_state_fix in H0; simpl in H0.
+    destruct H0 as [? [? [? [d' ?]]]].
+    inversion H1; subst; simpl.
+    - rewrite full_tree_equiv1 in H9.
+      rewrite H9.
+      apply IHtr1; [lia | | auto].
+      unfold list_on_tree_state; simpl.
+      unfold list_on_tree_state_fix; simpl.
+      inversion H0; subst.
+      split; [ | split; [ | split]].
+      * auto.
+      * eapply cons_partial_tree; eauto; simpl; rewrite Z.div_mul by lia;
+          [lia | lia | auto | auto].
+      * auto.
+      * exists d'; auto.
+    - pose proof complete_tree_pop_not_fullb _ _ H9.
+      replace (d - 1 - 1) with (d - 2) in H5 by lia.
+      rewrite H5.
+      apply IHtr2; [lia | | auto].
+      unfold list_on_tree_state; simpl.
+      unfold list_on_tree_state_fix; simpl.
+      inversion H0; subst.
+      split; [ | split; [ | split]].
+      * auto.
+      * pose proof Odd_Div2 n ltac:(lia).
+        eapply cons_partial_tree; eauto; simpl;
+          try rewrite H6; try lia; auto.
+        replace (n * 2 + 1 + -1) with (n * 2) by lia.
+        auto.
+      * auto.
+      * exists d'; auto.   
+Qed.
+
+Lemma complete_tree_pop_not_leaf: forall d t,
+  d >= 1 -> complete_tree_pop d t -> t <> Leaf.
+Proof.
+  intros.
+  induction H0; subst; simpl.
+  + lia.
+  + unfold not; intros; discriminate.
+  + unfold not; intros; discriminate.
+Qed.
+
+Lemma full_tree_not_leaf: forall d t,
+  d >= 1 -> full_tree_b d t = true -> t <> Leaf.
+Proof.
+  intros.
+  revert d H H0; induction t; simpl; intros.
+  + rewrite Z.eqb_eq in H0; lia.
+  + unfold not; intros; discriminate. 
+Qed.
+
+Lemma get_last_val_coincidence: forall d tr pt1 pt2,
+  complete_tree_pop d tr ->
+  tr <> Leaf ->
+  get_last_val (tree_to_partial_tree_pop_fix pt1 tr d) =
+  get_last_val (tree_to_partial_tree_pop_fix pt2 tr d).
+Proof.
+  intros.
+  revert d pt1 pt2 H.
+  induction tr; simpl; intros; [contradiction |].
+  inversion H; subst; simpl.
+  + rewrite full_tree_equiv1 in H5.
+    rewrite H5.
+    apply IHtr1; auto.
+    eapply complete_tree_pop_not_leaf; eauto.
+    rewrite <- full_tree_equiv1 in H5.
+    pose proof full_tree_nonneg _ _ H5.
+    lia.
+  + pose proof complete_tree_pop_not_fullb _ _ H5.
+    replace (d - 1 - 1) with (d - 2) in H1 by lia.
+    rewrite H1.
+    destruct (classic (tr2 = Leaf)).
+    1: { subst; simpl; auto. }
+    apply IHtr2; auto.
+Qed.
+
+Lemma list_on_tree_impl_state: forall (l: list Z) (ls rs: tree) (v: Z),
+  Zlength l > 2 -> list_on_tree l (Node v ls rs) ->
+  exists d, list_on_tree_state (firstn (Z.to_nat (Zlength l - 1)) (upd_Znth 1 l (Znth (Zlength l - 1) l)), 1) (nil, tree_cut_last ls rs d) /\  complete_tree_pop d (Node v ls rs).
+Proof.
+  intros.
+  unfold list_on_tree in H0.
+  destruct H0 as [? [? ?]].
+  rewrite <- complete_tree_equality in H2.
+  destruct H2 as [d].
+  exists d; split; [| auto].
+  unfold list_on_tree_state; simpl.
+  unfold list_on_tree_state_fix.
+  simpl.
+  split; [| split; [| split]].
+  2: {
+    apply nil_partial_tree; tauto.
+  }
+  1: {
+    unfold tree_cut_last.
+    inversion H2; subst.
+    + rewrite full_tree_equiv1 in H7.
+      rewrite H7.
+      apply list_nth_on_tree_Node.
+      - rewrite Zlength_firstn.
+        rewrite upd_Znth_Zlength by lia.
+        lia.
+      - rewrite Znth_firstn by lia.
+        rewrite upd_Znth_same by lia.
+        unfold tree_to_partial_tree_pop.
+        assert (Zlength l - 1 = last_index d 1 (Node v ls rs)). {
+          rewrite tree_last_index_size by auto; lia.
+        }
+        assert (ls <> Leaf). {
+          rewrite <- full_tree_equiv1 in H7.
+          pose proof full_tree_nonneg _ _ H7.
+          eapply complete_tree_pop_not_leaf; eauto; lia.
+        }
+        rewrite get_last_val_coincidence with (pt2 := (false, v, rs) :: nil); auto.
+        replace (tree_to_partial_tree_pop_fix [(false, v, rs)] ls (d - 1)) with (tree_to_partial_tree_pop_fix nil (Node v ls rs) d).
+        2: { simpl; rewrite H7; auto. }
+        erewrite list_on_tree_last_val; eauto.
+        * rewrite H3.
+          reflexivity.
+        * unfold list_on_tree_state; simpl.
+          unfold list_on_tree_state_fix; simpl.
+          split; [ | split; [ | split]].
+          -- auto.
+          -- apply nil_partial_tree; auto.
+          -- simpl in H1; lia. 
+          -- apply complete_tree_equality.
+             exists d; auto.
+      - admit.
+      - admit.
+    + pose proof complete_tree_pop_not_fullb _ _ H7.
+      replace (d - 1 - 1) with (d - 2) in H3 by lia.
+      rewrite H3.
+      apply list_nth_on_tree_Node.
+      - rewrite Zlength_firstn.
+        rewrite upd_Znth_Zlength by lia.
+        lia.
+      - rewrite Znth_firstn by lia.
+        rewrite upd_Znth_same by lia.
+        unfold tree_to_partial_tree_pop.
+        assert (rs <> Leaf). {
+          destruct (classic (ls = Leaf)).
+          + inversion H5; [ | rewrite H4 in H9; discriminate].
+            inversion H7.
+            2: { pose proof full_tree_nonneg _ _ H10; lia. }
+            2: { pose proof full_tree_nonneg _ _ H9; lia. }
+            subst.
+            simpl in H1; lia.
+        }
+        assert (Zlength l - 1 = last_index d 1 (Node v ls rs)). {
+          rewrite tree_last_index_size by auto; lia.
+        }
+        rewrite get_last_val_coincidence with (pt2 := (true, v, ls) :: nil); auto.
+        replace (get_last_val (tree_to_partial_tree_pop_fix [(true, v, ls)] rs (d - 1))) with (get_last_val (tree_to_partial_tree_pop_fix nil (Node v ls rs) d)).
+        2: { simpl; rewrite H3. auto. }
+        erewrite list_on_tree_last_val; eauto.
+        * rewrite H6.
+          reflexivity.
+        * unfold list_on_tree_state; simpl.
+          unfold list_on_tree_state_fix; simpl.
+          split; [ | split; [ | split]].
+          -- auto.
+          -- apply nil_partial_tree; auto.
+          -- simpl in H1; lia. 
+          -- apply complete_tree_equality.
+             exists d; auto.
+      - admit.
+      - admit. 
+  } 
+  
+Admitted.
+
+Lemma tree_not_emp: forall (t: tree),
+  tree_size t >= 1 -> exists v ls rs, t = Node v ls rs.
+Proof.
+  intros.
+  destruct t.
+  + simpl in H; lia. 
+  + exists v, t1, t2; reflexivity. 
+Qed.
+
+Lemma MaxHeap_tree_down_state: forall (ls rs: tree) (d v: Z),
+  MaxHeap (Node v ls rs) -> complete_tree_pop d (Node v ls rs) -> MaxHeap_tree_down ([], tree_cut_last ls rs d).
+Proof.
+Admitted.
+
+Lemma Pop_tree_list_rel: forall (l l': list Z) (t: tree),
+  list_on_tree l t -> heap_pop l l' -> MaxHeap t ->
+  exists t', list_on_tree l' t' /\ MaxHeap t' /\ tree_pop t t'.
+Proof.
+  intros.
+  unfold heap_pop in H0.
+  destruct H0.
+  + exists Leaf.
+    unfold list_on_tree in H.
+    destruct H, H2, H0.
+    unfold list_on_tree.
+    split.
+    * split; [apply list_nth_on_tree_Leaf|].
+      split; [simpl; lia|].
+      exists 1.
+      apply complete_tree_push_Leaf.
+      lia.
+    * split;[apply MaxHeap_Leaf; reflexivity|].
+      unfold tree_pop; left.
+      split;[lia|reflexivity].
+  + destruct H0.
+    destruct H2 as [pl].
+    remember H as H'; clear HeqH'.
+    unfold list_on_tree in H.
+    pose proof tree_not_emp t ltac:(lia).
+    destruct H3 as [v [ls [rs]]].
+    rewrite H3 in H'.
+    pose proof list_on_tree_impl_state _ _ _ _ H0 H'.
+    destruct H4 as [d].
+    destruct H4.
+    assert (Zlength (fst (firstn (Z.to_nat (Zlength l - 1))
+          (upd_Znth 1 l (Znth (Zlength l - 1) l)), 1)) >= 2). {
+      give_up.
+    }
+    pose proof Down_tree_list_rel _ _ _ H6 H4 H2.
+    subst.
+    pose proof MaxHeap_tree_down_state _ _ _ _ H1 H5.
+    specialize (H7 H3).
+    destruct H7 as [t'].
+    destruct H7, H8.
+    pose proof list_on_tree_state_impl_tree_compose _ _ H8.
+    simpl in H10.
+    exists (tree_compose (fst t') (snd t')).
+    split; [tauto|].
+    split; [tauto|].
+    unfold tree_pop; right.
+    exists v, ls, rs, t', d.
+    tauto.
+Admitted.
